coq/set/Core/Syntax.v
@@ -8,6 +8,11 @@ Inductive Formula : Type :=
 Definition Not (p:Formula)          :Formula := Imp p Bot.
 Definition Or  (p q:Formula)        :Formula := Imp (Not p) q.
 Definition And (p q:Formula)        :Formula := Not (Or (Not p) (Not q)).
-Definition Exist (n:nat) (p:Formula):Formula := Not (All n (Not p)).
+Definition Exi  (n:nat) (p:Formula) :Formula := Not (All n (Not p)).
+Definition Iff (p q:Formula)        :Formula := And (Imp p q) (Imp q p).
+Definition Sub (m n:nat)            :Formula := All 0 (Imp (Elem 0 m) (Elem 0 n)).
+Definition Equ (m n:nat)            :Formula := And
+    (All 0 (Iff (Elem 0 m) (Elem 0 n)))
+    (All 0 (Iff (Elem m 0) (Elem n 0))).
 
 
