coq/ref/CIC.v
@@ -23,29 +23,41 @@ Inductive isSort : Exp -> Prop :=
 
 (* Type for 'local declaration'                                                 *)
 Inductive LocalDecl : Type :=
-| LAssume : nat -> Exp -> LocalDecl         (* x:T , T is a type                *)
-| LDefine : nat -> Exp -> Exp -> LocalDecl  (* x := (t:T)                       *)
+| LAssume : nat -> Exp -> LocalDecl         (* n:T , T is a type                *)
+| LDefine : nat -> Exp -> Exp -> LocalDecl  (* n := (t:T)                       *)
 .
 
+(* Returns variable involved in given local declaration.                        *)
 Definition declVar (decl:LocalDecl) : nat :=
     match decl with
     | LAssume n _   => n
     | LDefine n _ _ => n
     end.
 
-(* variable involved must be distinct                                           *)
+(* Variable involved must be distinct                                           *)
 Definition LocalContext : Type := list LocalDecl. 
 
-Definition inLocCtx (n:nat) (ctx:LocalContext) : Prop := 
-    In n (map declVar ctx).
+Definition inLocCtx (n:nat) (C:LocalContext) : Prop := 
+    In n (map declVar C).
 
 Inductive GlobalDecl : Type :=
 | GAssume : nat -> Exp -> GlobalDecl        (* c:T, T is a type                 *)
 | GDefine : nat -> Exp -> Exp -> GlobalDecl (* c := t : T                       *)
-| GInduct : GlobalDecl                      (* TBT, define inductive objects    *)
+| GInduct : nat -> GlobalDecl               (* TBT, define inductive objects    *)
 .
+ 
+(* Returns constant involved in given global declaration.                       *)
+Definition declConst (decl:GlobalDecl) : nat :=
+    match decl with
+    | GAssume n _   => n
+    | GDefine n _ _ => n
+    | GInduct n     => n
+    end.
 
 Definition GlobalEnv : Type := list GlobalDecl.
+
+Definition inGblEnv (n:nat) (E:GlobalEnv) : Prop := 
+    In n (map declConst E).
 
 (* Judgement: E[C] |- t:T                                                       *)
 (* t is well-typed and has type T in the global env E and local context C       *)
@@ -57,19 +69,35 @@ Definition GlobalEnv : Type := list GlobalDecl.
 (* and a term T such that E[C] |- t:T can be derived from typing rules          *)
 
 Inductive Entails : GlobalEnv -> LocalContext -> Exp -> Exp -> Prop :=
-
-
+| AxProp: forall E C,
+    WF E C                      ->          (* WF(E)[C]                         *)
+    Entails E C EProp (EType 1)             (* E[C] |- Prop:Type(1)             *)
+| AxSet: forall E C,
+    WF E C                      ->          (* WF(E)[C]                         *)
+    Entails E C ESet (EType 1)              (* E[C] |- Set:Type(1)              *)
+| AxType: forall E C n,
+    WF E C                      ->          (* WF(E)[C]                         *)
+    Entails E C (EType n) (EType (S n))     (* E[C] |- Type(n):Type(n+1)        *)
 with WF : GlobalEnv -> LocalContext -> Prop :=  
 | WEmpty: WF [] []
-| WLocalAssume: forall env ctx T s n, 
-    Entails env ctx T s -> 
-    isSort s            -> 
-    ~ inLocCtx n ctx    -> 
-    WF env ((LAssume n T) :: ctx) 
-| WLocalDef: forall env ctx t T n,
-    Entails env ctx t T ->
-    ~ inLocCtx n ctx    ->
-    WF env ((LDefine n t T) :: ctx)
+| WLocalAssume: forall E C T s n, 
+    Entails E C T s             ->          (* E[C] |- T:s                      *)
+    isSort s                    ->          (* s is Prop, Set or Type(n)        *) 
+    ~ inLocCtx n C              ->          (* Var n not already in C           *)
+    WF E ((LAssume n T) :: C)               (* WF(E)[ (n:T) :: C]               *) 
+| WLocalDef: forall E C t T n,
+    Entails E C t T             ->          (* E[C] |- t:T                      *)
+    ~ inLocCtx n C              ->          (* Var n not already in C           *)
+    WF E ((LDefine n t T) :: C)             (* WF(E)[ (n := t:T) :: C ]         *)
+| WGlobalAssume: forall E T s n,         
+    Entails E [] T s            ->          (* E[[]] |- T:s                     *)
+    isSort s                    ->          (* s is Prop, Set or Type(n)        *)
+    ~ inGblEnv n E              ->          (* Const n not already in E         *)
+    WF ((GAssume n T) :: E) []              (* WF((n:T) :: E)[]                 *)
+| WGlobalDef: forall E t T n,
+    Entails E [] t T            ->          (* E[[]] |- t:T                     *)
+    ~ inGblEnv n E              ->          (* Const n not already in E         *)
+    WF ((GDefine n t T) :: E) []            (* WF((n := t:T) :: E)[]            *)                           
 .
 
 
