coq/set/Core/LEM.v
@@ -1,6 +1,6 @@
 Definition LEM : Prop :=  forall (p:Prop), p \/ ~p.
 
-Lemma LEMor : LEM -> forall (p q:Prop), (~p -> q) <-> p \/ q.
+Lemma LEMOr : LEM -> forall (p q:Prop), (~p -> q) <-> p \/ q.
 Proof.
     unfold LEM. intros L p q. split; intros H.
     - destruct (L p) as [H'|H'].
